{-# OPTIONS --without-K --rewriting #-}

open import Prelude
open import MiniUniverse
open import AbsoluteOpetopicTypes
open import DependentOpetopicType

module Sigma where

  Î£â‚’ : âˆ€ {â„“ â„“â†“} {n : â„•} (X : ğ•† â„“ n) (Xâ†“ : ğ•†â†“ â„“â†“ X) â†’ ğ•† (â„“-max â„“ â„“â†“) n

  fst-frm : âˆ€ {â„“ â„“â†“} {n : â„•} {X : ğ•† â„“ n} {Xâ†“ : ğ•†â†“ â„“â†“ X}
    â†’ Frm (Î£â‚’ X Xâ†“) â†’ Frm X

  snd-frm : âˆ€ {â„“ â„“â†“} {n : â„•} {X : ğ•† â„“ n} {Xâ†“ : ğ•†â†“ â„“â†“ X}
    â†’ (f : Frm (Î£â‚’ X Xâ†“)) â†’ Frmâ†“ Xâ†“ (fst-frm f)

  fst-cns : âˆ€ {â„“ â„“â†“} {n : â„•} {X : ğ•† â„“ n} {Xâ†“ : ğ•†â†“ â„“â†“ X}
    â†’ {f : Frm (Î£â‚’ X Xâ†“)} {P : â„™} {t : El P â†’ Frm (Î£â‚’ X Xâ†“)}
    â†’ (c : Cns (Î£â‚’ X Xâ†“) f P t)
    â†’ Cns X (fst-frm f) P (Î» p â†’ fst-frm (t p))

  snd-cns : âˆ€ {â„“ â„“â†“} {n : â„•} {X : ğ•† â„“ n} {Xâ†“ : ğ•†â†“ â„“â†“ X}
    â†’ {f : Frm (Î£â‚’ X Xâ†“)} {P : â„™} {t : El P â†’ Frm (Î£â‚’ X Xâ†“)}
    â†’ (c : Cns (Î£â‚’ X Xâ†“) f P t)
    â†’ Cnsâ†“ Xâ†“ (fst-cns c) (snd-frm f) (Î» p â†’ snd-frm (t p))

  Î£â‚’ {n = O} X Xâ†“ = Î£ X Xâ†“
  Î£â‚’ {n = S n} (Xâ‚™ , Xâ‚›â‚™) (Xâ†“â‚™ , Xâ†“â‚›â‚™) =
    Î£â‚’ Xâ‚™ Xâ†“â‚™ , Î» f â†’ Î£ (Xâ‚›â‚™ (fst-frm f)) (Î» x â†’ Xâ†“â‚›â‚™ (snd-frm f) x)

  fst-frm {n = O} {X = X} {Xâ†“ = Xâ†“} âŸª f , P , t âŸ« =
    âŸª fst f , P , (Î» p â†’ fst (t p)) âŸ«
  fst-frm {n = S n} {X = (Xâ‚™ , Xâ‚›â‚™)} {Xâ†“ = (Xâ†“â‚™ , Xâ†“â‚›â‚™)} (f , (x , xâ†“) , xâ‚›â‚™) =
    let fst-op = âŸª pos (opr xâ‚›â‚™) , (Î» p â†’ fst-frm (typ (opr xâ‚›â‚™) p)) , fst-cns (cns (opr xâ‚›â‚™)) âŸ«â‚’â‚š
    in fst-frm f , x , âŸª fst-op , (Î» p â†’ fst (dec xâ‚›â‚™ p)) âŸ«f

  snd-frm {n = O} {X = X} {Xâ†“ = Xâ†“} âŸª f , P , t âŸ« =
    snd f , Î» p â†’ snd (t p)
  snd-frm {n = S n} {X = X} {Xâ†“ = Xâ†“} (f , (x , xâ†“) , xâ‚›â‚™) =
    let snd-op = âŸª (Î» p â†’ snd-frm (typ (opr xâ‚›â‚™) p)) , snd-cns (cns (opr xâ‚›â‚™)) âŸ«â‚’â‚šâ†“ 
    in snd-frm f , xâ†“ , âŸª snd-op , (Î» p â†’ snd (dec xâ‚›â‚™ p)) âŸ«fâ†“

  fst-cns {n = O} c = tt
  fst-cns {n = S n} (lf f (x , xâ†“)) = {!lf (fst-frm f) x!}
  fst-cns {n = S n} (nd x fâ‚›â‚™ Î´ Îµ) = {!!}

  --
  -- So, fundamentally, we don't have:
  --   frm-frm (âŠ¤â‚š-Frm-rec f p) =/= âŠ¤â‚š-Frm-rec (fst-frm f) p
  --

  -- So I guess this would be solved by Î·-expansion in the mini
  -- universe.

  -- Hmmm.  But even after Î·-expansion we need:
  -- Î·-cns (fst-frm f) = fst-cns (Î·-cns f)

  -- Shit.  I thought we would get everything we needed.
  -- Okay, going to have to think more about this....

  snd-cns = {!!} 
