{-# OPTIONS --without-K --rewriting #-}

open import HoTT
open import Monad
open import MonadOver
open import Pb
open import OpetopicType
open import FundamentalThm
open import MonadEqv 
open import SliceUnfold
open import SliceAlgebraic

-- Can you fix this?
open import lib.NType2

module SliceUnique where

  -- Here, I believe is the proper coinductive statement
  -- of the theorem:

  alg‚Üì-unique : (M : ùïÑ) (M‚Üì : ùïÑ‚Üì M) (is-alg : is-algebraic M M‚Üì)
    ‚Üí (X : OpetopicType M) (is-fib : is-fibrant X)
    ‚Üí (ob‚âÉ : (i : Idx M) ‚Üí Idx‚Üì M‚Üì i ‚âÉ Ob X i)
    ‚Üí (witness : (i : Idx M) (c : Cns M i)
               ‚Üí (ŒΩ : (p : Pos M c) ‚Üí Ob X (Typ M c p))
               ‚Üí Ob (Hom X) ((i , ‚Äì> (ob‚âÉ i) (idx (contr-center (is-alg i c (Œª p ‚Üí <‚Äì (ob‚âÉ (Typ M c p)) (ŒΩ p)))))) , c , ŒΩ))
    ‚Üí ‚Üì-to-OpType M M‚Üì ‚âÉ‚Çí X 
  Ob‚âÉ (alg‚Üì-unique M M‚Üì is-alg X is-fib ob‚âÉ witness) = ob‚âÉ
  Hom‚âÉ (alg‚Üì-unique M M‚Üì is-alg X is-fib ob‚âÉ witness) =
    let open ExtUnfold M M‚Üì in
    alg‚Üì-unique ExtSlc‚ÇÅ ExtSlc‚Üì‚ÇÅ (slc-algebraic M M‚Üì)
      (op-transp (Slice‚âÉ (Pb‚âÉ' ob‚âÉ)) (Hom X))
      (op-transp-fib (Slice‚âÉ (Pb‚âÉ' ob‚âÉ)) (Hom X) (hom-fibrant is-fib))
      {!!}
      {!!}

  -- We are left with two proof obligations, which, after eliminating
  -- away the equivalence by univalence, become the following:

  module _ (M : ùïÑ) (M‚Üì : ùïÑ‚Üì M) (is-alg : is-algebraic M M‚Üì)
           -- (X‚ÇÄ : Rel‚ÇÄ M) (e : (i : Idx M) ‚Üí Idx‚Üì M‚Üì i ‚âÉ X‚ÇÄ i)
           (X‚ÇÅ : Rel‚ÇÅ M (Idx‚Üì M‚Üì)) (is-fib-X‚ÇÅ : is-fib‚ÇÅ M X‚ÇÅ)
           (X‚ÇÇ : Rel‚ÇÇ M X‚ÇÅ) (is-fib-X‚ÇÇ : is-fib‚ÇÇ M X‚ÇÇ)
           (witness : (i : Idx M) (c : Cns M i) (ŒΩ : (p : Pos M c) ‚Üí Idx‚Üì M‚Üì (Typ M c p))
                    ‚Üí X‚ÇÅ ((i , idx (contr-center (is-alg i c ŒΩ))) , (c , ŒΩ)))
           where

    open ExtUnfold M M‚Üì
    open import SliceAlg M M‚Üì

    -- The next equivalence is given generically by the
    -- fundamental theorem, which says both the spaces may
    -- be expressed as identity types.
    
    next-ob‚âÉ : (i : Idx ExtSlc‚ÇÅ) ‚Üí Idx‚Üì ExtSlc‚Üì‚ÇÅ i ‚âÉ X‚ÇÅ i
    next-ob‚âÉ ((i , j) , c , ŒΩ) = equiv to from to-from from-to

      -- Idx‚Üì ExtSlc‚Üì‚ÇÅ ((i , j) , c , ŒΩ)         ‚âÉ‚ü® {!!} ‚ü©  -- by the fundamental theorem
      -- j == idx (contr-center (is-alg i c ŒΩ))  ‚âÉ‚ü® {!!} ‚ü©  -- again, by the fundamental theorem, using "witness"
      -- X‚ÇÅ ((i , j) , c , ŒΩ) ‚âÉ‚àé

      where to : Idx‚Üì ExtSlc‚Üì‚ÇÅ ((i , j) , c , ŒΩ) ‚Üí X‚ÇÅ ((i , j) , c , ŒΩ)
            to ((j' , j'=j) , d , typ-d=ŒΩ) = transport (Œª x ‚Üí X‚ÇÅ ((i , x) , c , ŒΩ)) (ap idx alg=Œ± ‚àô' j'=j) (witness i c ŒΩ) 

              where Œ± : alg-comp M M‚Üì i c ŒΩ
                    Œ± = ‚ü¶ j' ‚à£ d ‚à£ Œª= typ-d=ŒΩ ‚üß 

                    alg=Œ± : contr-center (is-alg i c ŒΩ) == Œ±
                    alg=Œ± = contr-path (is-alg i c ŒΩ) Œ± 

            from : X‚ÇÅ ((i , j) , c , ŒΩ) ‚Üí Idx‚Üì ExtSlc‚Üì‚ÇÅ ((i , j) , c , ŒΩ)
            from x‚ÇÅ = (idx alg , fst= wit=x‚ÇÅ) , (cns alg , Œª p ‚Üí app= (typ alg) p) 

              where alg : alg-comp M M‚Üì i c ŒΩ
                    alg = contr-center (is-alg i c ŒΩ)
                    
                    wit=x‚ÇÅ : (idx (contr-center (is-alg i c ŒΩ)) , witness i c ŒΩ) == (j , x‚ÇÅ) 
                    wit=x‚ÇÅ = contr-has-all-paths ‚¶É is-fib-X‚ÇÅ i c ŒΩ ‚¶Ñ (idx (contr-center (is-alg i c ŒΩ)) , witness i c ŒΩ) (j , x‚ÇÅ) 

            -- So this is clear, but annoying because of the funext....
            to-from : (x‚ÇÅ : X‚ÇÅ ((i , j) , c , ŒΩ)) ‚Üí to (from x‚ÇÅ) == x‚ÇÅ
            to-from x‚ÇÅ = to (from x‚ÇÅ) =‚ü® idp ‚ü©                                                             -- defn
                         transport P (ap idx alg=Œ± ‚àô' fst= wit=x‚ÇÅ) (witness i c ŒΩ) =‚ü® {!idp!} ‚ü©            -- split
                         transport P (fst= wit=x‚ÇÅ) (transport P (ap idx alg=Œ±) (witness i c ŒΩ)) =‚ü® {!!} ‚ü©  -- because the first transport "is" the identity
                         transport P (fst= wit=x‚ÇÅ) (witness i c ŒΩ) =‚ü® to-transp (snd= wit=x‚ÇÅ) ‚ü©                               -- by wit=x‚ÇÅ below
                         x‚ÇÅ =‚àé 
  
                where P : Idx‚Üì M‚Üì i ‚Üí Set
                      P x = X‚ÇÅ ((i , x) , c , ŒΩ)
                      
                      alg : alg-comp M M‚Üì i c ŒΩ
                      alg = contr-center (is-alg i c ŒΩ)
                      
                      Œ± : alg-comp M M‚Üì i c ŒΩ
                      Œ± = ‚ü¶ idx alg ‚à£ cns alg ‚à£ Œª= (Œª p ‚Üí app= (typ alg) p) ‚üß 

                      alg=Œ± : contr-center (is-alg i c ŒΩ) == Œ±
                      alg=Œ± = contr-path (is-alg i c ŒΩ) Œ± 

                      wit=x‚ÇÅ : (idx (contr-center (is-alg i c ŒΩ)) , witness i c ŒΩ) == (j , x‚ÇÅ) 
                      wit=x‚ÇÅ = contr-has-all-paths ‚¶É is-fib-X‚ÇÅ i c ŒΩ ‚¶Ñ (idx (contr-center (is-alg i c ŒΩ)) , witness i c ŒΩ) (j , x‚ÇÅ) 

            from-to : (i‚ÇÅ : Idx‚Üì ExtSlc‚Üì‚ÇÅ ((i , j) , c , ŒΩ)) ‚Üí from (to i‚ÇÅ) == i‚ÇÅ
            from-to ((j' , j'=j) , d , typ-d=ŒΩ) = (idx alg , fst= wit=x‚ÇÅ) , (cns alg , Œª p ‚Üí app= (typ alg) p) =‚ü® {!!} ‚ü© -- because wit=x‚ÇÅ == with=x‚ÇÅ'
                                                  (idx alg , ap idx alg=Œ± ‚àô' j'=j) , (cns alg , Œª p ‚Üí app= (typ alg) p) =‚ü® {!!} ‚ü© -- should now be just from alg=Œ± ...
                                                  ((j' , j'=j) , d , typ-d=ŒΩ) =‚àé

                -- Yeah, so already here we see that this is kind of non-trivial and you're
                -- going to have to think about it a bit to make it work.  But, I mean, the
                -- existence of this equivalence is not really in doubt.  So you just have
                -- to work a bit more to unfold it and everything.

                where P : Idx‚Üì M‚Üì i ‚Üí Set
                      P x = X‚ÇÅ ((i , x) , c , ŒΩ)
                      
                      alg : alg-comp M M‚Üì i c ŒΩ
                      alg = contr-center (is-alg i c ŒΩ)

                      Œ± : alg-comp M M‚Üì i c ŒΩ
                      Œ± = ‚ü¶ j' ‚à£ d ‚à£ Œª= typ-d=ŒΩ ‚üß 

                      alg=Œ± : contr-center (is-alg i c ŒΩ) == Œ±
                      alg=Œ± = contr-path (is-alg i c ŒΩ) Œ± 

                      x‚ÇÅ : X‚ÇÅ ((i , j) , c , ŒΩ)
                      x‚ÇÅ = transport P (ap idx alg=Œ± ‚àô' j'=j) (witness i c ŒΩ) 

                      -- Okay, so this is an interesting idea.  Is it what you were looking for?
                      
                      wit=x‚ÇÅ : (idx (contr-center (is-alg i c ŒΩ)) , witness i c ŒΩ) == (j , x‚ÇÅ) 
                      wit=x‚ÇÅ = contr-has-all-paths ‚¶É is-fib-X‚ÇÅ i c ŒΩ ‚¶Ñ (idx (contr-center (is-alg i c ŒΩ)) , witness i c ŒΩ) (j , x‚ÇÅ) 

                      wit=x‚ÇÅ' : (idx (contr-center (is-alg i c ŒΩ)) , witness i c ŒΩ) == (j , x‚ÇÅ)
                      wit=x‚ÇÅ' = pair= (ap idx alg=Œ± ‚àô' j'=j) (from-transp P (ap idx alg=Œ± ‚àô' j'=j) idp) 



    is-fib-X‚ÇÅ' : is-fib‚ÇÅ M X‚ÇÅ
    is-fib-X‚ÇÅ' i c ŒΩ = has-level-in (ctr , pth) 

      where lcl‚âÉ : (j : Idx‚Üì M‚Üì i) ‚Üí Idx‚Üì ExtSlc‚Üì‚ÇÅ ((i , j) , c , ŒΩ) ‚âÉ X‚ÇÅ ((i , j) , c , ŒΩ)
            lcl‚âÉ j = next-ob‚âÉ ((i , j) , c , ŒΩ)

            the-eqv : alg-comp M M‚Üì i c ŒΩ ‚âÉ Œ£ (Idx‚Üì M‚Üì i) (Œª a ‚Üí X‚ÇÅ ((i , a) , c , ŒΩ))
            the-eqv = Œ£-emap-r lcl‚âÉ ‚àòe (alg-to-idx‚Üì M M‚Üì i c ŒΩ) 

            ctr : Œ£ (Idx‚Üì M‚Üì i) (Œª j ‚Üí X‚ÇÅ ((i , j) , (c , ŒΩ)))
            ctr = ‚Äì> (the-eqv) (contr-center (is-alg i c ŒΩ))

            pth : (y : Œ£ (Idx‚Üì M‚Üì i) (Œª j ‚Üí X‚ÇÅ ((i , j) , (c , ŒΩ)))) ‚Üí ctr == y
            pth y = ap (‚Äì> (the-eqv)) (contr-path (is-alg i c ŒΩ) (<‚Äì (the-eqv) y)) ‚àô
                    <‚Äì-inv-r (the-eqv) y  

    -- And here's what you wanted....
    two-fibs-agree : is-fib-X‚ÇÅ' == is-fib-X‚ÇÅ
    two-fibs-agree = prop-has-all-paths
      ‚¶É Œ†-level (Œª i ‚Üí Œ†-level (Œª c ‚Üí Œ†-level (Œª ŒΩ ‚Üí is-contr-is-prop))) ‚¶Ñ
        is-fib-X‚ÇÅ' is-fib-X‚ÇÅ

    -- Now.  This should give a relation between the two, right?  It should
    -- be possible to work out exactly what that relation is.  And I think
    -- you'll need that....

    -- Hmmm.  But the paths will be equal over the proof that the
    -- centers are equal. Aha!  But that's the key!  There will be
    -- such a proof by applying the function on either side.  Doesn't
    -- this already have to give a relation between the two?

    -- It may be useful, however, to prove the above equivalence
    -- directly so that we have better control over the image of
    -- various elements....

    -- In any case, we have now reduced ourselves to the following:
    -- we have to find a witness in X‚ÇÇ showing that it coincides
    -- with the proof that the slice is algebraic.  This should be
    -- carried out via induction, now with the extra hypothesis that
    -- X‚ÇÅ witnesses multiplication in the algebra.

    next-witness : (i : Idx ExtSlc‚ÇÅ) (œÉ : Cns ExtSlc‚ÇÅ i)
      ‚Üí (Œ∏ : (p : Pos ExtSlc‚ÇÅ œÉ) ‚Üí X‚ÇÅ (Typ ExtSlc‚ÇÅ œÉ p))
      ‚Üí X‚ÇÇ ((i , ‚Äì> (next-ob‚âÉ i) (slc-idx i œÉ (Œª p ‚Üí <‚Äì (next-ob‚âÉ (Typ ExtSlc‚ÇÅ œÉ p)) (Œ∏ p)))) , (œÉ , Œ∏))
    next-witness ((i , j) , ._ , ._) (lf .(i , j)) Œ∏ = transport (Œª x ‚Üí X‚ÇÇ ((((i , j) , Œ∑ M i , (Œª _ ‚Üí j)) , x) , lf (i , j) , Œ∏)) hence-need X‚ÇÇ-el

      where X‚ÇÅ-el : X‚ÇÅ ((i , j) , Œ∑ M i , (Œª _ ‚Üí j))
            X‚ÇÅ-el = fst (contr-center (is-fib-X‚ÇÇ ((i , j) , _ , _) (lf (i , j)) Œ∏))

            X‚ÇÇ-el : X‚ÇÇ ((((i , j) , Œ∑ M i , (Œª _ ‚Üí j)) , X‚ÇÅ-el) , lf (i , j) , Œ∏)
            X‚ÇÇ-el = snd (contr-center (is-fib-X‚ÇÇ ((i , j) , _ , _) (lf (i , j)) Œ∏))

            j' : Idx‚Üì M‚Üì i
            j' = idx (contr-center (is-alg i (Œ∑ M i) (Œª _ ‚Üí j)))

            X‚ÇÅ-wit : X‚ÇÅ ((i , j') , Œ∑ M i , (Œª _ ‚Üí j))
            X‚ÇÅ-wit = witness i (Œ∑ M i) (cst j)

            stronger-claim : contr-center (is-alg i (Œ∑ M i) (Œª _ ‚Üí j)) == ‚ü¶ j ‚à£ Œ∑‚Üì M‚Üì j ‚à£ Œª= (cst idp) ‚üß
            stronger-claim = contr-path (is-alg i (Œ∑ M i) (Œª _ ‚Üí j)) ‚ü¶ j ‚à£ Œ∑‚Üì M‚Üì j ‚à£ Œª= (cst idp) ‚üß 

            can-get : j , X‚ÇÅ-el == j' , X‚ÇÅ-wit
            can-get = contr-has-all-paths ‚¶É is-fib-X‚ÇÅ i (Œ∑ M i) (cst j) ‚¶Ñ (j , X‚ÇÅ-el) (j' , X‚ÇÅ-wit)

            hence-need : X‚ÇÅ-el == ‚Äì> (next-ob‚âÉ ((i , j) , Œ∑ M i , (Œª _ ‚Üí j))) ((j , idp) , Œ∑‚Üì M‚Üì j , (Œª _ ‚Üí idp))
            hence-need = X‚ÇÅ-el =‚ü® to-transp! (snd= can-get) ‚ü©
                         transport! P (fst= can-get) X‚ÇÅ-wit
                           =‚ü® {!!} ‚ü© -- Well, then clearly we need these two to be inverse to each other ...
                         transport P (ap idx stronger-claim) X‚ÇÅ-wit
                           =‚ü® idp ‚ü© 
                         ‚Äì> (next-ob‚âÉ ((i , j) , Œ∑ M i , (Œª _ ‚Üí j))) ((j , idp) , Œ∑‚Üì M‚Üì j , (Œª _ ‚Üí idp)) =‚àé

                where P : Idx‚Üì M‚Üì i ‚Üí Set
                      P x = X‚ÇÅ ((i , x) , Œ∑ M i , cst j)

            -- Well, maybe there is something simler.... from "can-get" we have
            -- that X‚ÇÅ-el == transport .... X‚ÇÅ-wit.  So if the equivalence is
            -- given as a transport in this way, wouldn't we be done?
            
            -- Interesting.  So it is a transport.  But using a
            -- different path.  There's the one given by X‚ÇÅ being
            -- fibrant, and the one given by the the fact that we are
            -- in an algebraic extension.

            -- Ohhh!  But I think that's it!  Because now I get *two*
            -- proofs that X‚ÇÅ is fibrant.  there's the one I have
            -- assumed, and there's the one given by pulling back the
            -- proof that the extension is algebraic along the
            -- equivalence.  What I need is that these two coincide.  But
            -- now I will get that because being fibrant is a property!
            -- And now I have that X‚ÇÅ is a transport via can-get and that
            -- it is a transport along a path which must be equivalent.

            -- Bam!!!


            -- Okay, so now we need to do something clever.  And here
            -- is where I think we need something like your argument
            -- from idempotence: any idempotent element must be
            -- equivalent to the canonical one.  But this time we have
            -- the extra information that the image of the idempotent
            -- element by the equivalence is the one claimed.

            -- Yes, something like this.  But there is likely to be
            -- another way to phrase this somehow.

            -- Okay, but we can define a "loop" to be an element like
            -- X‚ÇÅ-el.  And these will compose.  And so if my
            -- equivalence is a homomorphism (which I think it should
            -- be), I should be able to show that the thing on the
            -- right is idempotent.  But so is the thing on the left
            -- by fibrancy.  And therefore they should be equal and we
            -- get what we want.  That's the idea.

            -- Hmm.  But don't we still need to know that the
            -- multiplication defined by X‚ÇÇ and the one given by
            -- composition agree for this to work?


    next-witness ((i , j) , ._ , ._) (nd c Œ¥ Œµ) Œ∏ = {!!}

